cedar-lean/Cedar/SymCC/Symbolizer.lean
@@ -1,0 +1,244 @@
+/-
+ Copyright Cedar Contributors
+
+ Licensed under the Apache License, Version 2.0 (the "License");
+ you may not use this file except in compliance with the License.
+ You may obtain a copy of the License at
+
+      https://www.apache.org/licenses/LICENSE-2.0
+
+ Unless required by applicable law or agreed to in writing, software
+ distributed under the License is distributed on an "AS IS" BASIS,
+ WITHOUT WARRANTIES OR CONDITIONS OF ANY KIND, either express or implied.
+ See the License for the specific language governing permissions and
+ limitations under the License.
+-/
+
+import Cedar.SymCC.Env
+import Cedar.SymCC.Concretizer
+import Cedar.SymCC.Decoder
+import Cedar.Validation.Types
+
+/-!
+This file contains functions to encode a concrete `Env`
+into a `SymEnv`, which can also be thought of as an "inverse"
+of concretization.
+-/
+
+namespace Cedar.Spec
+
+open Data Spec SymCC Validation
+
+def Prim.symbolize : Prim → Term
+  | .bool b         => .prim (.bool b)
+  | .int i          => .prim (.bitvec i.toBitVec)
+  | .string s       => .prim (.string s)
+  | .entityUID euid => .prim (.entity euid)
+
+/-- Encodes a `Value` as a `Term` assuming it is of a certain type -/
+def Value.symbolize? (v : Value) (ty : CedarType) : Option Term :=
+  match v, ty with
+  | .prim p, _ => .some (Prim.symbolize p)
+  | .set s, .set ty => do
+    let elems := ← s.toList.mapM₁ (λ ⟨v, _⟩ => v.symbolize? ty)
+    .some (.set (Set.make elems) (TermType.ofType ty))
+  | .record rec, .record rty => do
+    let elems := ← rty.toList.mapM (λ (a, qty) => symbolizeAttr? rec a qty)
+    .some (Term.record (Map.mk elems))
+  | .ext e, _ => .some ↑e
+  | _, _ => .none
+termination_by sizeOf v
+decreasing_by
+  · cases s
+    rename_i h
+    have h := List.sizeOf_lt_of_mem h
+    simp [Set.toList, Set.elts] at h
+    simp [h]
+    omega
+  · simp
+where
+  symbolizeAttr? (rec : Map Attr Value) (a : Attr) (qty : QualifiedType) : Option (Attr × Term) :=
+    match _h : rec.find? a with
+    | .none => .some (a, .none (TermType.ofType qty.getType))
+    | .some v =>
+      match qty with
+      | .optional ty => do .some (a, .some (← v.symbolize? ty))
+      | .required ty => do .some (a, ← v.symbolize? ty)
+  termination_by sizeOf rec
+  decreasing_by
+    all_goals
+      have := Map.find?_mem_toList _h
+      have := List.sizeOf_lt_of_mem this
+      cases rec
+      simp [Map.toList, Map.kvs] at this ⊢
+      omega
+
+/--
+The variable ids here should match the variables in `SymRequest.ofRequestType`.
+-/
+def Request.symbolize? (req : Request) (Γ : TypeEnv) (var : TermVar) : Option Term :=
+  if var == { id := "principal", ty := TermType.ofType (.entity Γ.reqty.principal) } then
+    Value.symbolize? ↑req.principal (.entity Γ.reqty.principal)
+  else if var == { id := "action", ty := TermType.ofType (.entity Γ.reqty.action.ty) } then
+    Value.symbolize? ↑req.action (.entity Γ.reqty.action.ty)
+  else if var == { id := "resource", ty := TermType.ofType (.entity Γ.reqty.resource) } then
+    Value.symbolize? ↑req.resource (.entity Γ.reqty.resource)
+  else if var == { id := "context", ty := TermType.ofType (.record Γ.reqty.context) } then
+    Value.symbolize? ↑req.context (.record Γ.reqty.context)
+  else
+    .none
+
+def defaultEidOf (Γ : TypeEnv) (ety : EntityType) : String :=
+  -- TODO: Improve performance by looking up in `Γ` directly
+  Decoder.eidOfForEntities (SymEnv.ofEnv Γ).entities ety
+
+def defaultLitWithDefaultEid (Γ : TypeEnv) (ty : TermType) : Term :=
+  Decoder.defaultLit (defaultEidOf Γ) ty
+
+/--
+Generates an interpretation of the attribute map.
+-/
+def Entities.symbolizeAttrs?
+  (entities : Entities) (Γ : TypeEnv)
+  (ety : EntityType) (entry : EntitySchemaEntry)
+  (uuf : UUF) : Option UDF :=
+  if uuf == {
+    id := UUF.attrsId ety,
+    arg := TermType.ofType (.entity ety),
+    out := TermType.ofType (.record entry.attrs)
+  } then
+    .some udf
+  else
+    .none
+where
+  udf :=
+    let outTy := (.record entry.attrs)
+    {
+      arg := TermType.ofType (.entity ety),
+      out := TermType.ofType outTy,
+      -- Collect concrete attributes of every entity of type `ety`
+      table := Map.make (entities.toList.filterMap λ (euid, data) => do
+        if euid.ty = ety then
+          .some (↑euid, ← Value.symbolize? data.attrs outTy)
+        else
+          .none),
+      default := defaultLitWithDefaultEid Γ (TermType.ofType outTy),
+    }
+
+/--
+Generates interpretations for the tag key and value maps.
+-/
+def Entities.symbolizeTags?
+  (entities : Entities) (Γ : TypeEnv)
+  (ety : EntityType) (entry : EntitySchemaEntry)
+  (uuf : UUF) : Option UDF := do
+  let tagTy := ← entry.tags?
+  if uuf == {
+    id := UUF.tagKeysId ety,
+    arg := TermType.ofType (.entity ety),
+    out := TermType.ofType (.set .string),
+  } then
+    .some keysUDF
+  else if uuf == {
+    id := UUF.tagValsId ety,
+    arg := TermType.tagFor ety,
+    out := TermType.ofType tagTy,
+  } then
+    .some (valsUDF tagTy)
+  else
+    .none
+where
+  keysUDF := {
+    arg := TermType.ofType (.entity ety),
+    out := TermType.ofType (.set .string),
+    -- Collect concrete tag keys of every entity of type `ety`
+    table := Map.make (entities.toList.filterMap λ (euid, data) => do
+      if euid.ty = ety then
+        .some (↑euid, .set (Set.make (data.tags.keys.toList.map λ k => .prim (.string k))) .string)
+      else
+        .none),
+    default := defaultLitWithDefaultEid Γ (TermType.ofType (.set .string)),
+  }
+  valsUDF tagTy := {
+    arg := TermType.tagFor ety,
+    out := TermType.ofType tagTy,
+    -- Collect concrete tag values of every entity of type `ety`
+    -- i.e. a map from (entity, tag key) to tag value
+    table := Map.make (entities.toList.filterMap λ (uid, data) => do
+      if uid.ty = ety then
+        data.tags.toList.mapM λ (tag, value) => do
+          .some (
+            .record (Map.mk [
+              ("entity", .prim (.entity uid)),
+              ("tag", .prim (.string tag)),
+            ]),
+            ← Value.symbolize? value tagTy,
+          )
+      else
+        .none).flatten,
+    default := defaultLitWithDefaultEid Γ (TermType.ofType tagTy),
+  }
+
+/--
+Generates an interpretation for the ancestor map.
+-/
+def Entities.symbolizeAncs?
+  (entities : Entities) (Γ : TypeEnv)
+  (ety : EntityType) (entry : EntitySchemaEntry)
+  (uuf : UUF) : Option UDF :=
+  entry.ancestors.toList.findSome? λ ancTy =>
+    if uuf == {
+      id := UUF.ancsId ety ancTy,
+      arg := TermType.ofType (.entity ety),
+      out := TermType.ofType (.set (.entity ancTy)),
+    } then
+      .some (udf ancTy)
+    else
+      .none
+where
+  udf ancTy := {
+    arg := TermType.ofType (.entity ety),
+    out := TermType.ofType (.set (.entity ancTy)),
+    table := Map.make (entities.toList.filterMap λ (uid, data) => do
+    if uid.ty = ety then
+      .some (↑uid,
+        .set
+          (Set.make (data.ancestors.toList.filterMap λ anc =>
+            if anc.ty = ancTy then
+              .some (.prim (.entity anc))
+            else
+              .none))
+          (.entity ancTy))
+    else
+      .none),
+    default := defaultLitWithDefaultEid Γ (TermType.ofType (.set (.entity ancTy))),
+  }
+
+/--
+Symbolizes a concrete `Entities` into (part of) an `Interpretation` of `SymEnv.ofEnv Γ`.
+The `UUF` ids here should match those in `SymEntityData.ofStandardEntityType`.
+-/
+def Entities.symbolize? (entities : Entities) (Γ : TypeEnv) (uuf : UUF) : Option UDF :=
+  Γ.ets.toList.findSome? λ (ety, entry) =>
+    entities.symbolizeAttrs? Γ ety entry uuf <|>
+    entities.symbolizeTags? Γ ety entry uuf <|>
+    entities.symbolizeAncs? Γ ety entry uuf
+
+/--
+Converts an `Env` (assumed to be a well-typed instance of `TypeEnv`) into
+an `Interpretation` of `SymEnv.ofEnv Γ`.
+-/
+def Env.symbolize? (env : Env) (Γ : TypeEnv) : Interpretation :=
+  {
+    vars := λ var =>
+      match Request.symbolize? env.request Γ var with
+      | .some term => term
+      | .none => defaultLitWithDefaultEid Γ var.ty,
+    funs := λ uuf =>
+      match Entities.symbolize? env.entities Γ uuf with
+      | .some udf => udf
+      | .none => Decoder.defaultUDF (defaultEidOf Γ) uuf,
+    partials := λ t => defaultLitWithDefaultEid Γ t.typeOf,
+  }
+
+end Cedar.Spec
