cedar-lean/Cedar/Thm/SymCC/Data/UUF.lean
@@ -1,0 +1,69 @@
+/-
+ Copyright Cedar Contributors
+
+ Licensed under the Apache License, Version 2.0 (the "License");
+ you may not use this file except in compliance with the License.
+ You may obtain a copy of the License at
+
+      https://www.apache.org/licenses/LICENSE-2.0
+
+ Unless required by applicable law or agreed to in writing, software
+ distributed under the License is distributed on an "AS IS" BASIS,
+ WITHOUT WARRANTIES OR CONDITIONS OF ANY KIND, either express or implied.
+ See the License for the specific language governing permissions and
+ limitations under the License.
+-/
+
+import Cedar.SymCC.Env
+
+/-! Some facts about `UUF.*_id`s. -/
+
+namespace Cedar.Thm
+
+open Cedar.Thm
+open Cedar.Spec
+open Cedar.SymCC
+
+theorem uuf_attrs_ancs_no_confusion
+  {ety₁ ety₂ ancTy} :
+  UUF.attrsId ety₁ ≠ UUF.ancsId ety₂ ancTy
+:= by
+  apply String.ne_of_data_ne
+  simp [UUF.attrsId, UUF.ancsId, toString, String.data]
+
+theorem uuf_attrs_tag_keys_no_confusion
+  {ety₁ ety₂} :
+  UUF.attrsId ety₁ ≠ UUF.tagKeysId ety₂
+:= by
+  apply String.ne_of_data_ne
+  simp [UUF.attrsId, UUF.tagKeysId, toString, String.data]
+
+theorem uuf_attrs_tag_vals_no_confusion
+  {ety₁ ety₂} :
+  UUF.attrsId ety₁ ≠ UUF.tagValsId ety₂
+:= by
+  apply String.ne_of_data_ne
+  simp [UUF.attrsId, UUF.tagValsId, toString, String.data]
+
+theorem uuf_tag_vals_tag_keys_no_confusion
+  {ety₁ ety₂} :
+  UUF.tagValsId ety₁ ≠ UUF.tagKeysId ety₂
+:= by
+  apply String.ne_of_data_ne
+  simp [UUF.tagKeysId, UUF.tagValsId, toString, String.data]
+
+theorem uuf_tag_keys_ancs_no_confusion
+  {ety₁ ety₂ ancTy} :
+  UUF.tagKeysId ety₁ ≠ UUF.ancsId ety₂ ancTy
+:= by
+  apply String.ne_of_data_ne
+  simp [UUF.tagKeysId, UUF.ancsId, toString, String.data]
+
+theorem uuf_tag_vals_ancs_no_confusion
+  {ety₁ ety₂ ancTy} :
+  UUF.tagValsId ety₁ ≠ UUF.ancsId ety₂ ancTy
+:= by
+  apply String.ne_of_data_ne
+  simp [UUF.tagValsId, UUF.ancsId, toString, String.data]
+
+end Cedar.Thm
