cedar-lean/Cedar/Thm/SymCC/Env/Soundness.lean
@@ -1,0 +1,1781 @@
+/-
+ Copyright Cedar Contributors
+
+ Licensed under the Apache License, Version 2.0 (the "License");
+ you may not use this file except in compliance with the License.
+ You may obtain a copy of the License at
+
+      https://www.apache.org/licenses/LICENSE-2.0
+
+ Unless required by applicable law or agreed to in writing, software
+ distributed under the License is distributed on an "AS IS" BASIS,
+ WITHOUT WARRANTIES OR CONDITIONS OF ANY KIND, either express or implied.
+ See the License for the specific language governing permissions and
+ limitations under the License.
+-/
+
+import Cedar.Thm.Validation.Typechecker.Types
+import Cedar.Thm.SymCC.Concretizer
+import Cedar.Thm.SymCC.Symbolizer
+import Cedar.Thm.SymCC.Decoder
+import Cedar.Thm.SymCC.Env.ofEnv
+import Cedar.Thm.SymCC.Env.WF
+import Cedar.Thm.SymCC.Data.UUF
+import Cedar.SymCC.Concretizer
+import Cedar.SymCC.Symbolizer
+import Cedar.SymCC.Env
+
+/-!
+This file contains the soundness theorems of `Sym.ofEnv`
+-/
+
+namespace Cedar.Thm
+
+open Cedar.Thm
+open Cedar.Spec
+open Cedar.SymCC
+open Cedar.Validation
+open Cedar.Data
+
+private theorem env_symbolize?_same_request
+  {Γ : TypeEnv} {env : Env}
+  (hwf_env : env.StronglyWellFormed)
+  (hinst : InstanceOfWellFormedEnvironment env.request env.entities Γ) :
+  env.request ∼ ((SymEnv.ofEnv Γ).interpret (env.symbolize? Γ)).request
+:= by
+  have hwf := hinst.wf_env
+  simp only [
+    SymEnv.interpret,
+    Env.symbolize?,
+    SymEnv.ofEnv,
+    SymRequest.ofRequestType,
+    SymRequest.interpret,
+    Request.symbolize?,
+    Value.symbolize?,
+    Prim.symbolize,
+  ]
+  and_intros
+  all_goals
+    simp only [
+      beq_iff_eq, Option.bind_eq_bind,
+      Term.interpret, TermVar.mk.injEq,
+      String.reduceEq,
+      false_and, ↓reduceIte,
+    ]
+  -- Actions match
+  · have ⟨_, ⟨_, h, _, _⟩, _⟩ := hinst
+    simp [h]
+  -- Same context after interpretation
+  · have hwf_ctx_ty : (CedarType.record Γ.reqty.context).WellFormed Γ := by
+      have ⟨_, _, _, h⟩ := wf_env_implies_wf_request hwf
+      exact h
+    have hwt_ctx : InstanceOfType Γ env.request.context (.record Γ.reqty.context) := by
+      have ⟨_, ⟨_, _, _, h⟩, _⟩ := hinst
+      exact h
+    have hwf_ctx : (Value.record env.request.context).WellFormed env.entities := by
+      have ⟨⟨_, _, _, h⟩, _⟩ := hwf_env
+      exact h
+    have ⟨sym_ctx, hsym_ctx, hsame_sym_ctx⟩ := value?_symbolize?_id hwf hwf_ctx_ty hwf_ctx hwt_ctx
+    simp only [Value.symbolize?, Option.bind_eq_bind] at hsym_ctx
+
+    simp only [Option.bind_eq_bind, hsym_ctx]
+    exact hsame_sym_ctx
+
+private theorem env_symbolize?_lookup_attrs_udf
+  {Γ : TypeEnv} {env : Env}
+  {ety : EntityType} {entry : StandardSchemaEntry}
+  (hfind : Γ.ets.find? ety = .some (.standard entry)) :
+  (env.symbolize? Γ).funs {
+    id  := UUF.attrsId ety,
+    arg := TermType.ofType (.entity ety),
+    out := TermType.ofType (.record entry.attrs),
+  } = Entities.symbolizeAttrs?.udf env.entities Γ ety (EntitySchemaEntry.standard entry)
+:= by
+  simp only [Env.symbolize?, Entities.symbolize?]
+  rw [Map.map_toList_findSome? hfind _ _]
+  · intros kv hkv
+    have ⟨v, hv⟩ := hkv
+    simp [
+      Entities.symbolizeAttrs?,
+      Entities.symbolizeTags?,
+      uuf_attrs_tag_keys_no_confusion,
+      ne_comm.mp uuf_attrs_tag_keys_no_confusion,
+      uuf_tag_vals_tag_keys_no_confusion,
+      ne_comm.mp uuf_tag_vals_tag_keys_no_confusion,
+      uuf_attrs_tag_vals_no_confusion,
+      ne_comm.mp uuf_attrs_tag_vals_no_confusion,
+    ] at hv
+    cases hv with
+    | inl hv =>
+      have hv := hv.1.2.1
+      simp only [TermType.ofType, TermType.prim.injEq, TermPrimType.entity.injEq] at hv
+      simp [hv]
+    | inr hv =>
+      replace hv := hv.2
+      simp only [Entities.symbolizeAncs?] at hv
+      have ⟨_, _, _, _, h⟩ := List.findSome?_eq_some_iff.mp hv
+      simp [uuf_attrs_ancs_no_confusion] at h
+  · simp [Entities.symbolizeAttrs?, EntitySchemaEntry.attrs]
+
+private theorem env_symbolize?_lookup_tag_keys
+  {Γ : TypeEnv} {env : Env}
+  {ety : EntityType} {entry : StandardSchemaEntry}
+  {tagTy : CedarType}
+  (hfind : Γ.ets.find? ety = .some (.standard entry))
+  (htags : entry.tags = .some tagTy) :
+  (env.symbolize? Γ).funs {
+    id := UUF.tagKeysId ety,
+    arg := TermType.ofType (CedarType.entity ety),
+    out := TermType.ofType CedarType.string.set,
+  } = Entities.symbolizeTags?.keysUDF env.entities Γ ety
+:= by
+  simp only [Env.symbolize?, Entities.symbolize?]
+  rw [Map.map_toList_findSome? hfind _ _]
+  · intros kv hkv
+    have ⟨v, hv⟩ := hkv
+    simp [
+      Entities.symbolizeAttrs?,
+      Entities.symbolizeTags?,
+      ne_comm.mp uuf_attrs_tag_keys_no_confusion,
+      ne_comm.mp uuf_tag_vals_tag_keys_no_confusion,
+    ] at hv
+    cases hv with
+    | inl hv =>
+      simp only [bind, Option.bind] at hv
+      split at hv
+      contradiction
+      simp only [Option.ite_none_right_eq_some, Option.some.injEq] at hv
+      have hv := hv.1.2
+      simp only [TermType.ofType, TermType.prim.injEq, TermPrimType.entity.injEq] at hv
+      simp [hv]
+    | inr hv =>
+      replace hv := hv.2
+      simp only [Entities.symbolizeAncs?] at hv
+      have ⟨_, _, _, _, h⟩ := List.findSome?_eq_some_iff.mp hv
+      simp [uuf_tag_keys_ancs_no_confusion] at h
+  · simp [
+      Entities.symbolizeAttrs?,
+      Entities.symbolizeTags?,
+      EntitySchemaEntry.tags?,
+      htags,
+      ne_comm.mp uuf_attrs_tag_keys_no_confusion,
+    ]
+
+private theorem env_symbolize?_lookup_tag_vals
+  {Γ : TypeEnv} {env : Env}
+  {ety : EntityType} {tagTy : CedarType} {entry : StandardSchemaEntry}
+  (hfind : Γ.ets.find? ety = .some (.standard entry))
+  (hfind_tagTy : entry.tags = .some tagTy) :
+  (env.symbolize? Γ).funs {
+    id := UUF.tagValsId ety,
+    arg := TermType.tagFor ety,
+    out := TermType.ofType tagTy
+  } = Entities.symbolizeTags?.valsUDF env.entities Γ ety tagTy
+:= by
+  simp only [Env.symbolize?, Entities.symbolize?]
+  rw [Map.map_toList_findSome? hfind _ _]
+  · intros kv hkv
+    have ⟨v, hv⟩ := hkv
+    simp [
+      Entities.symbolizeAttrs?,
+      Entities.symbolizeTags?,
+      ne_comm.mp uuf_attrs_tag_keys_no_confusion,
+      ne_comm.mp uuf_attrs_tag_vals_no_confusion,
+      uuf_tag_vals_tag_keys_no_confusion,
+    ] at hv
+    cases hv with
+    | inl hv =>
+      simp only [bind, Option.bind] at hv
+      split at hv
+      contradiction
+      simp only [Option.ite_none_right_eq_some, Option.some.injEq] at hv
+      simp [hv.1]
+    | inr hv =>
+      replace hv := hv.2
+      simp only [Entities.symbolizeAncs?] at hv
+      have ⟨_, _, _, _, h⟩ := List.findSome?_eq_some_iff.mp hv
+      simp [uuf_tag_vals_ancs_no_confusion] at h
+  · simp [
+      Entities.symbolizeAttrs?,
+      Entities.symbolizeTags?,
+      ne_comm.mp uuf_attrs_tag_vals_no_confusion,
+      uuf_tag_vals_tag_keys_no_confusion,
+      hfind_tagTy,
+      EntitySchemaEntry.tags?,
+    ]
+
+private theorem env_symbolize?_lookup_ancs
+  {Γ : TypeEnv} {env : Env}
+  {ety : EntityType} {ancTy : EntityType}
+  {entry : StandardSchemaEntry}
+  (hfind : Γ.ets.find? ety = .some (.standard entry))
+  (hfind_ancTy : ancTy ∈ entry.ancestors) :
+  (env.symbolize? Γ).funs {
+    id := UUF.ancsId ety ancTy,
+    arg := TermType.ofType (CedarType.entity ety),
+    out := TermType.ofType (CedarType.entity ancTy).set,
+  } = Entities.symbolizeAncs?.udf env.entities Γ ety ancTy
+:= by
+  simp only [Env.symbolize?, Entities.symbolize?]
+  rw [Map.map_toList_findSome? hfind _ _]
+  · intros kv hkv
+    have ⟨v, hv⟩ := hkv
+    simp [
+      Entities.symbolizeAttrs?,
+      Entities.symbolizeTags?,
+      Entities.symbolizeAncs?,
+      ne_comm.mp uuf_attrs_tag_keys_no_confusion,
+      ne_comm.mp uuf_attrs_tag_vals_no_confusion,
+      ne_comm.mp uuf_attrs_ancs_no_confusion,
+      ne_comm.mp uuf_tag_keys_ancs_no_confusion,
+      ne_comm.mp uuf_tag_vals_ancs_no_confusion,
+      uuf_tag_vals_tag_keys_no_confusion,
+    ] at hv
+    have ⟨_, _, _, _, h, _⟩ := List.findSome?_eq_some_iff.mp hv
+    split at h
+    · rename_i heq
+      have heq := heq.2.1
+      simp only [TermType.ofType] at heq
+      simp only [TermType.prim.injEq, TermPrimType.entity.injEq] at heq
+      simp [heq]
+    · contradiction
+  · simp [
+      Entities.symbolizeAttrs?,
+      Entities.symbolizeTags?,
+      Entities.symbolizeAncs?,
+      ne_comm.mp uuf_attrs_tag_vals_no_confusion,
+      ne_comm.mp uuf_attrs_ancs_no_confusion,
+      ne_comm.mp uuf_tag_keys_ancs_no_confusion,
+      ne_comm.mp uuf_tag_vals_ancs_no_confusion,
+    ]
+    apply List.findSome?_unique hfind_ancTy
+    · intros ancTy' hancTy'_mem
+      simp only [
+        Option.ite_none_right_eq_some,
+        Option.some.injEq,
+        exists_and_left, exists_eq',
+        and_true,
+      ] at hancTy'_mem
+      have heq := hancTy'_mem.2
+      simp only [
+        TermType.ofType, TermType.set.injEq,
+        TermType.prim.injEq,
+        TermPrimType.entity.injEq,
+      ] at heq
+      simp [heq]
+    · simp
+
+/--
+For simplifying `Factory.app` on some of the `UDF`s in `Env.symbolize?`.
+-/
+private theorem map_make_filterMap_find?
+  [BEq α] [BEq β] [LawfulBEq α] [LawfulBEq β]
+  [DecidableEq γ] [LT γ] [DecidableLT γ] [StrictLT γ]
+  {m : Map α β}
+  {k : α} {v : β} {k' : γ} {v' : κ}
+  {f : α × β → Option (γ × κ)}
+  (hfind : m.find? k = .some v)
+  (hkv : f (k, v) = .some (k', v'))
+  (hf : ∀ kv, (∃ v'', f kv = .some (k', v'')) → kv.1 = k) :
+  (Map.make (m.toList.filterMap f)).find? k' = .some v'
+:= by
+  apply Map.find?_implies_make_find?
+  simp only [List.find?_filterMap]
+  have :
+    List.find? (fun a => Option.any (fun x => x.fst == k') (f a)) m.toList
+    = .some (k, v)
+  := by
+    apply Map.map_find?_implies_find?_weaker_pred hfind
+    · intros kv h
+      simp only [Option.any] at h
+      split at h
+      · rename_i f_out heq
+        simp at h
+        apply hf kv
+        exists f_out.snd
+        simp only [heq, ←h]
+      · contradiction
+    · simp [
+        Option.any,
+        hkv,
+      ]
+  simp [this, hkv]
+
+/--
+For simplifying `Factory.app` on some of the `UDF`s in `Env.symbolize?`.
+-/
+private theorem map_make_filterMap_flatten_find?
+  [BEq α] [BEq β] [LawfulBEq α] [LawfulBEq β]
+  [DecidableEq γ] [LT γ] [DecidableLT γ] [StrictLT γ]
+  {m : Map α β}
+  {k : α} {v : β} {k' : γ} {v' : κ}
+  {f : α × β → Option (List (γ × κ))}
+  (hfind : m.find? k = .some v)
+  (hkv : ∃ l, f (k, v) = .some l ∧ l.find? (λ x => x.1 == k') = .some (k', v'))
+  (hf : ∀ kv, (∃ l, f kv = .some l ∧ (l.find? (λ x => x.1 == k')).isSome) → kv.1 = k) :
+  (Map.make (m.toList.filterMap f).flatten).find? k' = .some v'
+:= by
+  apply Map.find?_implies_make_find?
+  simp only [List.find?_flatten]
+  cases m with | mk l =>
+  simp only [Map.toList, Map.kvs, Map.find?] at *
+  split at hfind
+  rotate_left; contradiction
+  rename_i heq
+  simp only [Option.some.injEq] at hfind
+  simp only [hfind] at heq
+  have := List.find?_some heq
+  simp only [beq_iff_eq] at this
+  simp only [this] at heq
+  induction l with
+  | nil => contradiction
+  | cons hd tl ih =>
+    simp only [List.find?] at heq
+    split at heq
+    · simp only [Option.some.injEq] at heq
+      have ⟨fkv, hfkv, hfind_fkv⟩ := hkv
+      simp only [List.filterMap, heq, hfkv]
+      simp only [List.findSome?, hfind_fkv]
+    · rename_i hne_hd_key
+      simp only [List.filterMap]
+      split
+      · exact ih heq
+      · rename_i l' hhd
+        simp only [beq_eq_false_iff_ne, ne_eq] at hne_hd_key
+        have := hf hd
+        have :
+          (∃ l, f hd = some l ∧ (List.find? (fun x => x.fst == k') l).isSome = true) → False
+        := by
+          intros h
+          apply hne_hd_key
+          apply this h
+        simp only [
+          beq_iff_eq, Prod.exists,
+          exists_and_right, exists_eq_right,
+          imp_false, not_exists, not_and,
+        ] at this
+        have hfind_l' := this l' hhd
+        simp only [List.findSome?]
+        split
+        · rename_i heq
+          simp only [heq] at hfind_l'
+          simp at hfind_l'
+        · exact ih heq
+
+private theorem app_table_make_filterMap
+  [BEq α] [BEq β] [LawfulBEq α] [LawfulBEq β]
+  {arg : TermType} {out : TermType} {default : Term}
+  {m : Map α β} {k : α} {v : β}
+  {t : Term} {r : Term}
+  {f : α × β → Option (Term × Term)}
+  (hfind : m.find? k = .some v)
+  (hkv : f (k, v) = .some (t, r))
+  (hf : ∀ kv, (∃ v'', f kv = .some (t, v'')) → kv.1 = k)
+  (hlit : t.isLiteral) :
+  Factory.app
+    (.udf {
+      arg := arg,
+      out := out,
+      table := Map.make (m.toList.filterMap f),
+      default := default,
+    }) t
+  = r
+:= by
+  simp only [
+    Factory.app,
+    UnaryFunction.interpret,
+    hlit,
+    ↓reduceIte,
+  ]
+  have := map_make_filterMap_find? hfind hkv hf
+  simp only [this, Option.some.injEq]
+
+private theorem env_symbolize?_same_entity_data_standard_same_tag
+  {Γ : TypeEnv} {env : Env}
+  {uid : EntityUID} {data : EntityData} {entry : StandardSchemaEntry}
+  (hwf_env : env.StronglyWellFormed)
+  (hinst : InstanceOfWellFormedEnvironment env.request env.entities Γ)
+  (hinst_data : InstanceOfEntitySchemaEntry uid data Γ)
+  (hfind_entry : Map.find? Γ.ets uid.ty = some (.standard entry))
+  (hfind_data : Map.find? env.entities uid = some data) :
+  SameTags uid data
+    (SymEntityData.interpret
+      (env.symbolize? Γ)
+      (SymEntityData.ofStandardEntityType uid.ty entry))
+:= by
+  have ⟨_, ⟨hwf_entities, _⟩⟩ := hwf_env
+  have ⟨hwf_data_attrs, _, _, hwf_data_tags_map, hwf_data_tags⟩ := hwf_entities.2 uid data hfind_data
+  have ⟨hwf_Γ, _, _⟩ := hinst
+  have ⟨entry', hfind_entry', _, hwt_data_attrs, hwt_data_ancs, hwt_data_tags⟩ := hinst_data
+  simp only [hfind_entry, Option.some.injEq] at hfind_entry'
+  simp only [←hfind_entry', EntitySchemaEntry.attrs] at hwt_data_attrs hwt_data_tags
+  simp only [
+    SymEntityData.ofStandardEntityType,
+    SymEntityData.interpret,
+  ]
+  simp only [
+    SameTags,
+    SymEntityData.ofStandardEntityType.symTags,
+  ]
+  cases hentry_tags : entry.tags with
+  | none =>
+    simp only [Option.map_none]
+    simp only [InstanceOfEntityTags, EntitySchemaEntry.tags?, hentry_tags] at hwt_data_tags
+    exact hwt_data_tags
+  | some tagTy =>
+    have happ_tag_keys :
+      Factory.app (UnaryFunction.udf (Entities.symbolizeTags?.keysUDF env.entities Γ uid.ty)) (Term.entity uid)
+      = .set (Set.make (data.tags.keys.toList.map λ k => .prim (.string k))) .string
+    := by
+      apply app_table_make_filterMap hfind_data
+      · simp
+      · simp
+      · simp [Term.isLiteral]
+    have hkeys_set_is_literal :
+      (Term.set
+        (Set.make (List.map (fun k => Term.prim (TermPrim.string k)) data.tags.keys.toList))
+        TermType.string).isLiteral
+    := by
+      unfold Term.isLiteral
+      apply List.all_eq_true.mpr
+      intros x hmem_x
+      have hmem_x := x.property
+      have := (Set.make_mem _ _).mpr hmem_x
+      have ⟨_, _, hx⟩ := List.mem_map.mp this
+      simp [←hx, Term.isLiteral]
+    simp only [Option.map_some]
+    constructor
+    -- Tag key exists iff the symbolic tag key is true
+    · intros tag
+      simp only [
+        SymTags.hasTag,
+        SymTags.interpret,
+        UnaryFunction.interpret,
+        SymEntityData.ofStandardEntityType.symTags,
+        env_symbolize?_lookup_tag_keys hfind_entry hentry_tags,
+      ]
+      simp only [happ_tag_keys, Factory.set.member]
+      constructor
+      · intros hno_tag
+        split
+        · rfl
+        · rename_i s _ hs_not_emp heq
+          simp only [Term.set.injEq] at heq
+          replace heq := heq.1
+          simp only [
+            Term.isLiteral, hkeys_set_is_literal, Bool.and_self,
+            ↓reduceIte, Term.prim.injEq,
+            TermPrim.bool.injEq,
+          ]
+          simp only [←heq]
+          have :
+            ¬((Set.make (List.map (fun k => Term.prim (TermPrim.string k)) data.tags.keys.toList)).contains (Term.string tag) = true)
+          := by
+            intros h
+            have := Set.contains_prop_bool_equiv.mp h
+            have := (Set.make_mem _ _).mpr this
+            have ⟨_, hmem, heq⟩ := List.mem_map.mp this
+            simp only [Term.prim.injEq, TermPrim.string.injEq] at heq
+            simp only [heq] at hmem
+            have ⟨_, hfind⟩ := Map.in_keys_exists_value hmem
+            have := (Map.in_list_iff_find?_some hwf_data_tags_map).mp hfind
+            simp only [hno_tag] at this
+            contradiction
+          simp only [this]
+        · rename_i h
+          have := h
+            (Set.make (List.map (fun k => Term.prim (TermPrim.string k)) data.tags.keys.toList))
+            TermType.string
+            rfl
+          contradiction
+      · split
+        · rename_i heq
+          simp only [Term.set.injEq] at heq
+          replace heq := heq.1
+          simp only [forall_const]
+          have :
+            List.map (fun k => Term.prim (TermPrim.string k)) data.tags.keys.toList = []
+          := by
+            apply (Set.make_empty _).mpr
+            simp [heq, Set.isEmpty, Set.empty]
+          have := List.map_eq_nil_iff.mp this
+          have := Map.map_keys_empty_implies_map_empty this
+          simp only [this, Map.find?, List.find?]
+        · rename_i s _ _ heq
+          simp only [Term.set.injEq] at heq
+          replace heq := heq.1
+          simp only [
+            Term.isLiteral, hkeys_set_is_literal,
+            Bool.and_self, ↓reduceIte,
+            Term.prim.injEq, TermPrim.bool.injEq,
+          ]
+          simp only [←heq]
+          intros hnot_contains
+          have {v} (h : data.tags.find? tag = .some v) :
+            False
+          := by
+            have :
+              Term.string tag ∈ Set.make (List.map (fun k => Term.prim (TermPrim.string k)) data.tags.keys.toList)
+            := by
+              apply (Set.make_mem _ _).mp
+              apply List.mem_map.mpr
+              exists tag
+              simp only [and_true]
+              apply Map.in_list_in_keys
+              apply (Map.in_list_iff_find?_some hwf_data_tags_map).mpr h
+            have := Set.not_contains_prop_bool_equiv.mp hnot_contains this
+            contradiction
+          cases h : data.tags.find? tag with
+          | none => rfl
+          | some =>
+            have := this h
+            contradiction
+        · rename_i h
+          have := h
+            (Set.make (List.map (fun k => Term.prim (TermPrim.string k)) data.tags.keys.toList))
+            TermType.string
+            rfl
+          contradiction
+    -- Tag values match
+    · intros tag val hfind_tag
+      constructor
+      · simp only [
+          SymTags.hasTag,
+          SymTags.interpret,
+          UnaryFunction.interpret,
+          SymEntityData.ofStandardEntityType.symTags,
+          env_symbolize?_lookup_tag_keys hfind_entry hentry_tags,
+        ]
+        simp only [
+          happ_tag_keys,
+          Factory.set.member,
+        ]
+        split
+        · rename_i heq
+          simp only [Term.set.injEq] at heq
+          replace heq := heq.1
+          have :
+            List.map (fun k => Term.prim (TermPrim.string k)) data.tags.keys.toList = []
+          := by
+            apply (Set.make_empty _).mpr
+            simp [heq, Set.isEmpty, Set.empty]
+          have := List.map_eq_nil_iff.mp this
+          have := Map.map_keys_empty_implies_map_empty this
+          simp [this, Map.find?, List.find?] at hfind_tag
+        · rename_i s _ _ heq
+          simp only [Term.set.injEq] at heq
+          replace heq := heq.1
+          simp only [
+            Term.isLiteral, hkeys_set_is_literal,
+            Bool.and_self, ↓reduceIte,
+            Term.prim.injEq, TermPrim.bool.injEq,
+          ]
+          simp only [←heq]
+          simp only [Set.contains_prop_bool_equiv]
+          apply (Set.make_mem _ _).mp
+          apply List.mem_map.mpr
+          exists tag
+          simp only [and_true]
+          apply Map.in_list_in_keys
+          apply (Map.in_list_iff_find?_some hwf_data_tags_map).mpr hfind_tag
+        · rename_i h
+          have := h
+            (Set.make (List.map (fun k => Term.prim (TermPrim.string k)) data.tags.keys.toList))
+            TermType.string
+            rfl
+          contradiction
+      · simp only [
+          SymEntityData.ofStandardEntityType.symTags,
+          SymTags.interpret,
+          SymTags.getTag!,
+          UnaryFunction.interpret,
+          env_symbolize?_lookup_tag_vals hfind_entry hentry_tags,
+          Entities.symbolizeTags?.valsUDF,
+          SameValues,
+        ]
+        have hwf_val := hwf_data_tags tag val hfind_tag
+        simp only [InstanceOfEntityTags, EntitySchemaEntry.tags?, hentry_tags] at hwt_data_tags
+        have hwt_val := hwt_data_tags val (Map.find?_some_implies_in_values hfind_tag)
+        have hwf_tagTy : tagTy.WellFormed Γ
+        := by
+          apply wf_env_implies_wf_tag_type hwf_Γ (ety := uid.ty)
+          simp only [EntitySchema.tags?, hfind_entry, Option.map, EntitySchemaEntry.tags?]
+          congr
+        have ⟨sym_val, hsym_val, hval_sym_val⟩ := value?_symbolize?_id hwf_Γ hwf_tagTy hwf_val hwt_val
+        simp only [←hval_sym_val]
+        congr
+        simp only [
+          Factory.app, Factory.tagOf,
+          Term.isLiteral, List.cons.sizeOf_spec,
+          Prod.mk.sizeOf_spec,
+          Term.prim.sizeOf_spec,
+          TermPrim.entity.sizeOf_spec,
+          TermPrim.string.sizeOf_spec,
+          List.nil.sizeOf_spec, List.attach₃,
+          List.pmap, List.all_cons,
+          List.all, Bool.and_self,
+          ↓reduceIte, Option.bind_eq_bind,
+        ]
+        rw [map_make_filterMap_flatten_find? (v' := sym_val) hfind_data]
+        · simp
+          have hsym_tag_val_id :
+            ∀ tag val,
+              (tag, val) ∈ data.tags.toList →
+              ∃ sym_val,
+                val.symbolize? tagTy = .some sym_val ∧
+                sym_val.value? = .some val
+          := by
+            intros tag val hmem_tag_val
+            have hfind_tag_val := (Map.in_list_iff_find?_some hwf_data_tags_map).mp hmem_tag_val
+            have hwf_tag_val := hwf_data_tags _ _ hfind_tag_val
+            have hwt_tag_val := hwt_data_tags _ (Map.find?_some_implies_in_values hfind_tag_val)
+            exact value?_symbolize?_id hwf_Γ hwf_tagTy hwf_tag_val hwt_tag_val
+          have ⟨sym_tags, hsym_tags⟩ :
+            ∃ sym_tags,
+              data.tags.toList.mapM
+                (λ x => do
+                  some (
+                    Term.record (Map.mk [
+                      ("entity", Term.prim (TermPrim.entity uid)),
+                      ("tag", Term.prim (TermPrim.string x.fst)),
+                    ]),
+                    ← x.snd.symbolize? tagTy))
+              = .some sym_tags
+          := by
+            apply List.all_some_implies_mapM_some
+            intros tag_val hmem_tag_val
+            have ⟨sym_tag_val, hsym_tag_val, hval_sym_tag_val⟩ := hsym_tag_val_id tag_val.1 tag_val.2 hmem_tag_val
+            simp [hsym_tag_val]
+          exists sym_tags
+          simp only [Option.bind_eq_bind] at hsym_tags
+          simp only [hsym_tags, true_and]
+          apply List.find?_unique_entry
+          · simp only [beq_iff_eq, Prod.forall, Prod.mk.injEq]
+            intros tag' val' hmem_tag'_val' htag'
+            have ⟨_, _, h⟩ := List.mapM_some_implies_all_from_some hsym_tags (tag', val') hmem_tag'_val'
+            rename_i tag_val' hmem_tag_val'
+            simp only [
+              bind, Option.bind,
+            ] at h
+            split at h
+            contradiction
+            simp only [Option.some.injEq, Prod.mk.injEq] at h
+            simp only [
+              ←h.1, Term.record.injEq, Map.mk.injEq,
+              List.cons.injEq, Prod.mk.injEq,
+              Term.prim.injEq, TermPrim.string.injEq,
+              true_and, and_true,
+            ]
+            rename_i heq
+            simp only [h.2] at heq
+            have ⟨sym_val', h₁, h₂⟩ := hsym_tag_val_id tag_val'.1 tag_val'.2 hmem_tag_val'
+            have heq_tag : tag_val'.fst = tag
+            := by
+              simp only [htag'] at h
+              replace h := h.1
+              simp only [
+                Term.record.injEq, Map.mk.injEq, List.cons.injEq, Prod.mk.injEq,
+                Term.prim.injEq, TermPrim.string.injEq, true_and, and_true,
+              ] at h
+              exact h
+            have heq_val : tag_val'.snd = val
+            := by
+              have := (Map.in_list_iff_find?_some hwf_data_tags_map).mp hmem_tag_val'
+              simp only [heq_tag, hfind_tag, Option.some.injEq] at this
+              simp [this]
+            simp only [heq_val, hsym_val, Option.some.injEq] at heq
+            simp [heq_tag, heq]
+          · have := (Map.in_list_iff_find?_some hwf_data_tags_map).mpr hfind_tag
+            have ⟨y, hmem_y, hy⟩ := List.mapM_some_implies_all_some hsym_tags (tag, val) this
+            simp only [hsym_val, Option.bind_some, Option.some.injEq] at hy
+            simp only [←hy] at hmem_y
+            exact hmem_y
+          · simp
+        · intros kv hkv
+          have ⟨l, h₁, h₂⟩ := hkv
+          simp only [Option.ite_none_right_eq_some] at h₁
+          replace h₁ := h₁.2
+          have ⟨x, hmem_x, hx⟩ := List.find?_isSome.mp h₂
+          have ⟨_, _, h⟩ := List.mapM_some_implies_all_from_some h₁ x hmem_x
+          simp only [bind, Option.bind] at h
+          split at h
+          contradiction
+          simp only [Option.some.injEq] at h
+          simp only [←h] at hx
+          simp only [
+            beq_iff_eq, Term.record.injEq, Map.mk.injEq,
+            List.cons.injEq, Prod.mk.injEq,
+            Term.prim.injEq, TermPrim.entity.injEq, true_and,
+            TermPrim.string.injEq, and_true,
+          ] at hx
+          exact hx.1
+
+private theorem env_symbolize?_same_entity_data_standard
+  {Γ : TypeEnv} {env : Env}
+  {uid : EntityUID} {data : EntityData} {entry : StandardSchemaEntry}
+  (hwf_env : env.StronglyWellFormed)
+  (hinst : InstanceOfWellFormedEnvironment env.request env.entities Γ)
+  (hinst_data : InstanceOfEntitySchemaEntry uid data Γ)
+  (hfind_entry : Map.find? Γ.ets uid.ty = some (.standard entry))
+  (hfind_data : Map.find? env.entities uid = some data) :
+  SameEntityData uid data
+    (SymEntityData.interpret
+      (env.symbolize? Γ)
+      (SymEntityData.ofStandardEntityType uid.ty entry))
+:= by
+  have ⟨_, ⟨hwf_entities, _⟩⟩ := hwf_env
+  have ⟨hwf_data_attrs, _, hwf_data_ancs, hwf_data_tags, _⟩ := hwf_entities.2 uid data hfind_data
+  have ⟨hwf_Γ, _, _⟩ := hinst
+  have ⟨entry', hfind_entry', _, hwt_data_attrs, hwt_data_ancs, hwt_data_tags⟩ := hinst_data
+  simp only [hfind_entry, Option.some.injEq] at hfind_entry'
+  simp only [←hfind_entry', EntitySchemaEntry.attrs] at hwt_data_attrs hwt_data_ancs hwt_data_tags
+  simp only [
+    SymEntityData.ofStandardEntityType,
+    SymEntityData.interpret,
+  ]
+  -- Proof obgligations of `SameEntityData`
+  and_intros
+  · simp only [
+      SymEntityData.ofStandardEntityType.attrsUUF,
+      UnaryFunction.interpret,
+      env_symbolize?_lookup_attrs_udf hfind_entry,
+      Entities.symbolizeAttrs?.udf,
+      SameValues,
+    ]
+    have hwf_attrs_ty : (CedarType.record entry.attrs).WellFormed Γ
+    := by
+      have : Γ.ets.attrs? uid.ty = some entry.attrs := by
+        simp [EntitySchema.attrs?, hfind_entry, EntitySchemaEntry.attrs]
+      apply wf_env_implies_wf_attrs hwf_Γ this
+    have ⟨sym_attrs, hsym_attrs, hval_sym_attrs⟩ := value?_symbolize?_id hwf_Γ hwf_attrs_ty hwf_data_attrs hwt_data_attrs
+    simp only [←hval_sym_attrs]
+    congr
+    apply app_table_make_filterMap hfind_data
+    · simp [EntitySchemaEntry.attrs, hsym_attrs]
+    · intros kv hkv
+      simp only [
+        EntitySchemaEntry.attrs, Option.bind_eq_bind,
+        Option.ite_none_right_eq_some,
+        exists_and_left,
+        bind, Option.bind,
+      ] at hkv
+      replace ⟨_, ⟨_, hkv⟩⟩ := hkv
+      split at hkv
+      · contradiction
+      · rename_i heq
+        simp only [Option.some.injEq, Prod.mk.injEq, Term.prim.injEq, TermPrim.entity.injEq] at hkv
+        simp [hkv.1]
+    · simp [Term.isLiteral]
+  · intros anc hmem_anc
+    simp only [SameEntityData.InSymAncestors]
+    have hfind_ancTy := hwt_data_ancs anc hmem_anc
+    simp only [EntitySchemaEntry.ancestors] at hfind_ancTy
+    exists UnaryFunction.interpret (env.symbolize? Γ) (SymEntityData.ofStandardEntityType.ancsUUF uid.ty anc.ty)
+    constructor
+    · apply Map.find?_mapOnValues_some
+      apply Map.find?_implies_make_find?
+      simp only [List.find?_map]
+      unfold Function.comp
+      simp only
+      have : List.find? (λ x => x == anc.ty) entry.ancestors.toList = .some anc.ty
+      := by apply List.mem_implies_find? hfind_ancTy <;> simp
+      simp only [this, Option.map]
+    · simp only [
+        SymEntityData.ofStandardEntityType.ancsUUF,
+        UnaryFunction.interpret,
+        env_symbolize?_lookup_ancs hfind_entry hfind_ancTy,
+        Entities.symbolizeAncs?.udf,
+      ]
+      exists (Set.make (List.filterMap
+        (λ anc' =>
+          if anc'.ty = anc.ty then
+            .some (.prim (.entity anc'))
+          else
+            .none)
+        data.ancestors.toList))
+      constructor
+      · apply app_table_make_filterMap hfind_data
+        · simp
+        · simp
+        · simp only [Term.isLiteral]
+      · apply (Set.make_mem _ _).mp
+        apply List.mem_filterMap.mpr
+        exists anc
+        constructor
+        · exact hmem_anc
+        · simp
+  · simp only
+    intros ancTy ancUF hancUF
+    simp only [
+      SameEntityData.InAncestors,
+    ]
+    have ⟨uuf, huuf, hancUF⟩ := Map.find?_mapOnValues_some' _ hancUF
+    have := (Map.in_list_iff_find?_some (Map.make_wf _)).mpr huuf
+    have := Map.make_mem_list_mem this
+    have ⟨_, hmem_ancTy, heq⟩ := List.mem_map.mp this
+    simp only [Prod.mk.injEq] at heq
+    replace huuf := heq.2
+    simp only [heq.1] at huuf hmem_ancTy
+    simp only [←huuf] at hancUF
+    simp only [
+      hancUF,
+      SymEntityData.ofStandardEntityType.ancsUUF,
+      UnaryFunction.interpret,
+      env_symbolize?_lookup_ancs hfind_entry hmem_ancTy,
+      Entities.symbolizeAncs?.udf,
+    ]
+    exists (Set.make (List.filterMap
+      (λ anc =>
+        if anc.ty = ancTy then
+          .some (.prim (.entity anc))
+        else
+          .none)
+      data.ancestors.toList))
+    constructor
+    · apply app_table_make_filterMap hfind_data
+      · simp
+      · simp
+      · simp only [Term.isLiteral]
+    · intros anc_term hmem_anc_term
+      have := (Set.make_mem _ _).mpr hmem_anc_term
+      have ⟨anc', hmem_anc', heq⟩ := List.mem_filterMap.mp this
+      exists anc'
+      simp only [Option.ite_none_right_eq_some, Option.some.injEq] at heq
+      simp only [←heq, true_and]
+      exact hmem_anc'
+  · exact env_symbolize?_same_entity_data_standard_same_tag
+      hwf_env hinst hinst_data hfind_entry hfind_data
+
+private theorem env_symbolize?_same_entity_data_enum
+  {Γ : TypeEnv} {env : Env}
+  {uid : EntityUID} {data : EntityData} {eids : Set String}
+  (hinst : InstanceOfWellFormedEnvironment env.request env.entities Γ)
+  (hinst_data : InstanceOfEntitySchemaEntry uid data Γ)
+  (hfind_entry : Map.find? Γ.ets uid.ty = some (.enum eids)) :
+  SameEntityData uid data
+    (SymEntityData.interpret
+      (env.symbolize? Γ)
+      (SymEntityData.ofEnumEntityType uid.ty eids))
+:= by
+  have ⟨hwf_Γ, _, _⟩ := hinst
+  have ⟨entry', hfind_entry', _, hwt_data_attrs, hwt_data_ancs, hwt_data_tags⟩ := hinst_data
+  simp only [hfind_entry, Option.some.injEq] at hfind_entry'
+  simp only [←hfind_entry'] at hwt_data_attrs hwt_data_ancs hwt_data_tags
+  simp only [
+    SymEntityData.interpret,
+    SymEntityData.ofEnumEntityType,
+  ]
+  have hemp_data_ancs : data.ancestors = (Set.mk [])
+  := by
+    simp only [EntitySchemaEntry.ancestors, Set.empty] at hwt_data_ancs
+    cases h : data.ancestors with | mk ancs =>
+    cases ancs with
+    | nil => rfl
+    | cons anc ancs =>
+      simp only [h] at hwt_data_ancs
+      have : anc ∈ Set.mk (anc :: ancs) := by
+        apply Set.mem_cons_self
+      have := hwt_data_ancs anc this
+      contradiction
+  -- Proof obgligations of `SameEntityData`
+  and_intros
+  · simp only [
+      SymEntityData.emptyAttrs,
+      UnaryFunction.interpret,
+      Factory.app,
+      Term.isLiteral,
+      ↓reduceIte,
+      Map.empty,
+      Map.find?,
+      List.find?
+    ]
+    simp only [EntitySchemaEntry.attrs, Map.empty] at hwt_data_attrs
+    cases hwt_data_attrs with | instance_of_record rec rty h₁ h₂ h₃ =>
+    have hemp_data_attrs : data.attrs = (Map.mk [])
+    := by
+      cases h : data.attrs with | mk attrs =>
+      cases attrs with
+      | nil => rfl
+      | cons attr attrs =>
+        simp only [h] at h₁
+        have := h₁ attr.1
+        simp [Map.contains, Map.find?, List.find?] at this
+    simp [
+      hemp_data_attrs,
+      SameValues,
+      Term.value?,
+      List.mapM₂,
+      List.attach₂,
+    ]
+  · simp only [hemp_data_ancs]
+    intros anc hmem_anc
+    contradiction
+  · intros ancTy ancUF
+    simp [Map.empty, Map.mapOnValues, List.map, Map.find?, List.find?]
+  · simp only [SameTags, Option.map_none]
+    simp only [InstanceOfEntityTags, EntitySchemaEntry.tags?] at hwt_data_tags
+    exact hwt_data_tags
+
+private theorem env_symbolize?_same_entities_ordinary
+  {Γ : TypeEnv} {env : Env}
+  {uid : EntityUID} {data : EntityData}
+  (hwf_env : env.StronglyWellFormed)
+  (hinst : InstanceOfWellFormedEnvironment env.request env.entities Γ)
+  (hinst_data : InstanceOfEntitySchemaEntry uid data Γ)
+  (hfind_data : Map.find? env.entities uid = some data) :
+  ∃ δ,
+    Map.find?
+      (SymEnv.interpret (env.symbolize? Γ) (SymEnv.ofEnv Γ)).entities
+      uid.ty = some δ ∧
+    SameEntityData uid data δ
+:= by
+  have ⟨hwf_Γ, _, _⟩ := hinst
+  have ⟨entry, hfind_entry, _⟩ := hinst_data
+  have := ofSchema_find?_ets hfind_entry
+  simp only [
+    SymEnv.interpret,
+    SymEnv.ofEnv,
+    SymEntities.interpret,
+    SymEntities.ofSchema,
+  ]
+  have hfind_interp_entry :
+    (Map.mapOnValues
+      (SymEntityData.interpret (env.symbolize? Γ))
+      (Map.make
+        (
+          List.map (λ x => (x.fst, SymEntityData.ofEntityType x.fst x.snd)) (Map.toList Γ.ets) ++
+          List.map
+            (λ actTy =>
+              (actTy,
+                SymEntityData.ofActionType actTy (List.map (λ x => x.fst.ty) (Map.toList Γ.acts)).eraseDups
+                  Γ.acts))
+            (List.map (λ x => x.fst.ty) (Map.toList Γ.acts)).eraseDups
+        )
+      )
+    ).find? uid.ty = .some (SymEntityData.interpret (env.symbolize? Γ) (SymEntityData.ofEntityType uid.ty entry))
+  := by
+    simp only [← Map.find?_mapOnValues, Option.map_eq_some_iff]
+    exists SymEntityData.ofEntityType uid.ty entry
+  simp only [hfind_interp_entry, Option.some.injEq, exists_eq_left']
+  simp only [SymEntityData.ofEntityType]
+  have hwf_entry := wf_env_implies_wf_entity_entry hwf_Γ hfind_entry
+  cases entry with
+  | standard entry =>
+    simp only
+    exact env_symbolize?_same_entity_data_standard hwf_env hinst hinst_data hfind_entry hfind_data
+  | enum es =>
+    simp only
+    exact env_symbolize?_same_entity_data_enum hinst hinst_data hfind_entry
+
+private theorem env_symbolize?_same_entities_action
+  {Γ : TypeEnv} {env : Env}
+  {uid : EntityUID} {data : EntityData}
+  (hinst : InstanceOfWellFormedEnvironment env.request env.entities Γ)
+  (hinst_data : InstanceOfActionSchemaEntry uid data Γ) :
+  ∃ δ,
+    Map.find?
+      (SymEnv.interpret (env.symbolize? Γ) (SymEnv.ofEnv Γ)).entities
+      uid.ty = some δ ∧
+    SameEntityData uid data δ
+:= by
+  have ⟨hwf_Γ, _, _⟩ := hinst
+  have ⟨hattrs_emp, htags_emp, ⟨entry, hfind_entry, heq_ancs⟩⟩ := hinst_data
+  simp only [
+    SymEnv.interpret,
+    SymEntities.interpret,
+    SymEnv.ofEnv,
+  ]
+  simp only [←(Map.find?_mapOnValues _ _ _)]
+  have hwf_acts := wf_env_implies_wf_acts_map hwf_Γ
+  have := ofSchema_find?_acts hwf_Γ hfind_entry
+  simp only [this, Option.map_some, Option.some.injEq, exists_eq_left']
+  simp only [
+    SymEntityData.ofActionType,
+    SymEntityData.interpret,
+    UnaryFunction.interpret,
+    SymEntityData.emptyAttrs,
+    Option.map,
+  ]
+  -- Simplifying terms like `(SymEntityData.ofActionType.ancsUDF _ _).table.find? ...`
+  have hf_ancs_find {ancTy : EntityType} :
+    (Map.make
+      (List.filterMap
+        (λ x : EntityUID × ActionSchemaEntry =>
+          (SymEntityData.ofActionType.termOfType? uid.ty x.fst).bind
+          λ t => some (t, SymEntityData.ofActionType.ancsTerm ancTy x.snd.ancestors.toList))
+        (Map.toList Γ.acts))).find?
+      (Term.prim (TermPrim.entity uid))
+    = .some (.set
+      (Set.make (List.filterMap (SymEntityData.ofActionType.termOfType? ancTy) entry.ancestors.toList))
+      (TermType.entity ancTy))
+  := by
+    apply Map.find?_implies_make_find?
+    simp only [List.find?_filterMap]
+    have :
+      (List.find?
+        (λ a => Option.any
+          (λ x => x.fst == Term.prim (TermPrim.entity uid))
+          ((SymEntityData.ofActionType.termOfType? uid.ty a.fst).bind
+            λ t => some (t, SymEntityData.ofActionType.ancsTerm ancTy a.snd.ancestors.toList)))
+        (Map.toList Γ.acts))
+      = .some (uid, entry)
+    := by
+      apply List.find?_unique_entry
+      · intros x hmem_x hfilter
+        simp only [
+          SymEntityData.ofActionType.termOfType?,
+          Option.any,
+        ] at hfilter
+        split at hfilter
+        · rename_i v hv
+          split at hv
+          · rename_i heq_ty
+            simp only [Option.bind_some, Option.some.injEq] at hv
+            cases v
+            rename_i v₁ v₂
+            simp only [beq_iff_eq] at hfilter
+            simp only [
+              hfilter,
+              Prod.mk.injEq, Term.prim.injEq,
+              TermPrim.entity.injEq,
+            ] at hv
+            cases x
+            rename_i x₁ x₂
+            have := (Map.in_list_iff_find?_some hwf_acts).mp hmem_x
+            simp only at hv
+            simp only [hv.1] at this
+            simp only [hfind_entry, Option.some.injEq] at this
+            simp only [←this, hv.1]
+          · contradiction
+        · contradiction
+      · exact (Map.in_list_iff_find?_some hwf_acts).mpr hfind_entry
+      · simp [
+          SymEntityData.ofActionType.termOfType?,
+        ]
+    simp only [this, Option.bind_some]
+    simp [
+      SymEntityData.ofActionType.termOfType?,
+      SymEntityData.ofActionType.ancsTerm,
+      Factory.setOf,
+        TermType.ofType,
+    ]
+  -- Prove obligations of `SameEntityData`
+  and_intros
+  · simp only [
+      Factory.app,
+      Map.empty,
+      Map.find?,
+      List.find?,
+      Term.isLiteral,
+      ↓reduceIte,
+    ]
+    simp [
+      hattrs_emp,
+      SameValues,
+      Term.value?,
+      List.attach₂,
+      List.mapM₂,
+      Map.empty,
+    ]
+  -- Same ancestor map
+  · intros anc hmem_anc
+    simp only [SameEntityData.InSymAncestors]
+    simp only [←(Map.find?_mapOnValues _ _ _)]
+    have :
+      (Map.make
+        (List.map
+          (λ ancTy => (ancTy, SymEntityData.ofActionType.ancsUDF uid.ty Γ.acts ancTy))
+          (List.map (λ x => x.fst.ty)
+            (Map.toList Γ.acts)).eraseDups)).find?
+          anc.ty
+      = .some (SymEntityData.ofActionType.ancsUDF uid.ty Γ.acts anc.ty)
+    := by
+      apply Map.make_map_values_find
+      apply List.mem_implies_mem_eraseDups
+      apply List.mem_map.mpr
+      simp only [heq_ancs] at hmem_anc
+      have ⟨anc_entry, hfind_anc, _⟩ := wf_env_implies_wf_action_entity_ancestor hwf_Γ hfind_entry hmem_anc
+      exists (anc, anc_entry)
+      constructor
+      · apply (Map.in_list_iff_find?_some hwf_acts).mpr
+        exact hfind_anc
+      · simp
+    simp only [this]
+    simp only [
+      Option.map, UnaryFunction.interpret,
+      SymEntityData.ofActionType.ancsUDF,
+      Option.bind_eq_bind, Option.some.injEq,
+      exists_eq_left',
+      Factory.app,
+      Term.isLiteral,
+      ↓reduceIte,
+    ]
+    -- generalize hf_ancs_term : (λ x : EntityUID × ActionSchemaEntry =>
+    --   (SymEntityData.ofActionType.termOfType? uid.ty x.fst).bind
+    --   fun t => some (t, SymEntityData.ofActionType.ancsTerm anc.ty x.snd.ancestors.toList)) = f_ancs_term
+    exists Set.make (entry.ancestors.toList.filterMap
+      (SymEntityData.ofActionType.termOfType? anc.ty))
+    simp only [hf_ancs_find, true_and]
+    apply (Set.make_mem _ _).mp
+    apply List.mem_filterMap.mpr
+    exists anc
+    constructor
+    · simp only [heq_ancs] at hmem_anc
+      exact hmem_anc
+    · simp only [SymEntityData.ofActionType.termOfType?, ↓reduceIte]
+  · simp only
+    intros ancTy ancUF hancUF
+    have hancUF :
+      ancUF = SymEntityData.ofActionType.ancsUDF uid.ty Γ.acts ancTy
+    := by
+      simp only [←Map.find?_mapOnValues] at hancUF
+      simp only [Option.map_eq_some_iff] at hancUF
+      have ⟨ancUF', hancUF', heq_ancUF⟩ := hancUF
+      have := Map.find?_mem_toList hancUF'
+      have := Map.make_mem_list_mem this
+      have ⟨_, _, h⟩ := List.mem_map.mp this
+      simp only [Prod.mk.injEq] at h
+      simp only [h.1, true_and] at h
+      simp only [h]
+      simp only [←h] at heq_ancUF
+      simp only [UnaryFunction.interpret] at heq_ancUF
+      split at heq_ancUF
+      · rename_i heq
+        simp only [SymEntityData.ofActionType.ancsUDF] at heq
+        contradiction
+      · rename_i heq
+        simp only [h] at heq
+        simp only [heq_ancUF] at heq
+        simp [heq]
+    simp only [
+      SameEntityData.InAncestors,
+      hancUF,
+      Factory.app,
+      SymEntityData.ofActionType.ancsUDF,
+      Term.isLiteral,
+      ↓reduceIte,
+    ]
+    simp only [Option.bind_eq_bind, hf_ancs_find, Term.set.injEq, and_true, exists_eq_left']
+    intros anc_term hmem_anc_term
+    have hmem_anc_term := (Set.make_mem _ _).mpr hmem_anc_term
+    have ⟨anc, hmem_anc, hanc_term⟩ := List.mem_filterMap.mp hmem_anc_term
+    exists anc
+    simp only [
+      SymEntityData.ofActionType.termOfType?,
+      Option.ite_none_right_eq_some,
+      Option.some.injEq,
+    ] at hanc_term
+    simp only [hanc_term.2, true_and, heq_ancs]
+    exact hmem_anc
+  · simp only [SameTags, htags_emp]
+
+private theorem env_symbolize?_same_entities
+  {Γ : TypeEnv} {env : Env}
+  (hwf_env : env.StronglyWellFormed)
+  (hinst : InstanceOfWellFormedEnvironment env.request env.entities Γ) :
+  env.entities ∼ ((SymEnv.ofEnv Γ).interpret (env.symbolize? Γ)).entities
+:= by
+  intros uid data hfind_uid_data
+  have ⟨hwf_Γ, _, ⟨hinst_data, _⟩⟩ := hinst
+  specialize hinst_data uid data hfind_uid_data
+  cases hinst_data with
+  | inl hinst_data =>
+    exact env_symbolize?_same_entities_ordinary hwf_env hinst hinst_data hfind_uid_data
+  | inr hinst_data =>
+    exact env_symbolize?_same_entities_action hinst hinst_data
+
+private theorem defaultLitWithDefaultEid_wf
+  {Γ : TypeEnv} {ty : TermType}
+  (hwf_Γ : Γ.WellFormed)
+  (hwf_ty : ty.WellFormed (SymEnv.ofEnv Γ).entities) :
+  (defaultLitWithDefaultEid Γ ty).WellFormed (SymEnv.ofEnv Γ).entities
+:= by
+  apply default_lit_wf hwf_ty
+  intros ety hety
+  simp only [SymEntities.isValidEntityType, Map.contains, Option.isSome] at hety
+  split at hety
+  · rename_i δ hfind_δ
+    simp only [SymEntities.isValidEntityUID, hfind_δ, defaultEidOf, Decoder.eidOfForEntities]
+    split
+    · rename_i eids hmembers
+      -- simp only [hmembers]
+      split
+      · rename_i eid _ _ hhead
+        simp only [Option.some.injEq] at hhead
+        simp only [hhead, Option.some.injEq] at hmembers
+        simp [←hmembers, Set.contains, Set.elts, hhead]
+      · rename_i hempty_eids
+        replace hempty_eids : eids = (Set.mk []) := by
+          cases eids with | mk eids' =>
+          cases eids' with
+          | nil => rfl
+          | cons eid rst =>
+            have := hempty_eids δ.attrs δ.ancestors eid rst δ.tags
+            simp [←hmembers] at this
+        -- `eids` should not be empty
+        simp only [SymEnv.ofEnv, SymEntities.ofSchema] at hfind_δ
+        have := Map.make_mem_list_mem (Map.find?_mem_toList hfind_δ)
+        have := List.mem_append.mp this
+        cases this with
+        | inl hmem_ets =>
+          have ⟨⟨ety', entry'⟩, hmem_ety', h⟩ := List.mem_map.mp hmem_ets
+          simp only [Prod.mk.injEq] at h
+          cases entry' with
+          | standard =>
+            replace h := h.2
+            simp only [
+              SymEntityData.ofEntityType,
+              SymEntityData.ofStandardEntityType,
+            ] at h
+            simp only [←h] at hmembers
+            contradiction
+          | enum eids' =>
+            simp only [
+              ←h.2, h.1,
+              SymEntityData.ofEntityType,
+              SymEntityData.ofEnumEntityType,
+              Option.some.injEq,
+              hempty_eids,
+            ] at hmembers
+            have := (Map.in_list_iff_find?_some (wf_env_implies_wf_ets_map hwf_Γ)).mp hmem_ety'
+            have := wf_env_implies_wf_entity_entry hwf_Γ this
+            simp only [EntitySchemaEntry.WellFormed, Bool.not_eq_true] at this
+            have h := this.2
+            simp [hmembers, Set.isEmpty, Set.empty] at h
+        | inr hmem_acts =>
+          have ⟨ety', hmem_ety', h⟩ := List.mem_map.mp hmem_acts
+          simp only [Prod.mk.injEq] at h
+          simp only [
+            ←h.2, h.1,
+            SymEntityData.ofActionType,
+            SymEntityData.ofActionType.acts,
+            Option.some.injEq,
+            hempty_eids,
+          ] at hmembers
+          have hemp :
+            List.filterMap (fun x => if x.fst.ty = ety then some x.fst.eid else none) (Map.toList Γ.acts)
+            = []
+          := by
+            apply (Set.make_empty _).mpr
+            simp only [Set.isEmpty, Set.empty, beq_iff_eq, hmembers]
+          have := List.mem_eraseDups_implies_mem hmem_ety'
+          have ⟨act, hmem_act, hact_ty⟩ := List.mem_map.mp this
+          simp only [h.1] at hact_ty
+          have := List.filterMap_empty_iff_all_none.mp hemp act hmem_act
+          simp only [hact_ty, ↓reduceIte] at this
+          contradiction
+    · rfl
+  · contradiction
+
+private theorem env_symbolize?_wf_vars
+  {Γ : TypeEnv} {env : Env} {var : TermVar}
+  (hwf_env : env.StronglyWellFormed)
+  (hinst : InstanceOfWellFormedEnvironment env.request env.entities Γ)
+  (hwf_var : TermVar.WellFormed (SymEnv.ofEnv Γ).entities var) :
+  Interpretation.WellFormed.WellFormedVarInterpretation
+    (SymEnv.ofEnv Γ).entities
+    var
+    ((env.symbolize? Γ).vars var)
+:= by
+  have ⟨⟨hwf_princ, hwf_action, hwf_resource, hwf_context⟩, _⟩ := hwf_env
+  have ⟨hwf_Γ, _, _⟩ := hinst
+  have ⟨hwf_princ_ty, hcontains_action, hwf_resource_ty, hwf_context_ty⟩ := wf_env_implies_wf_request hwf_Γ
+  replace hwf_princ_ty :
+    (CedarType.entity Γ.reqty.principal).WellFormed Γ
+  := by constructor; exact hwf_princ_ty
+  replace hwf_resource_ty :
+    (CedarType.entity Γ.reqty.resource).WellFormed Γ
+  := by constructor; exact hwf_resource_ty
+  have hwf_action_ty :
+    (CedarType.entity Γ.reqty.action.ty).WellFormed Γ
+  := by
+    constructor
+    apply Or.inr
+    simp only [ActionSchema.IsActionEntityType]
+    exists Γ.reqty.action
+  have ⟨_, ⟨hinst_princ, hinst_action, hinst_resource, hinst_context⟩, _⟩ := hinst
+  replace hinst_princ :
+    InstanceOfType Γ (Value.prim (Prim.entityUID env.request.principal)) (CedarType.entity Γ.reqty.principal)
+  := by constructor; exact hinst_princ
+  replace hinst_resource :
+    InstanceOfType Γ (Value.prim (Prim.entityUID env.request.resource)) (CedarType.entity Γ.reqty.resource)
+  := by constructor; exact hinst_resource
+  replace hinst_action :
+    InstanceOfType Γ (Value.prim (Prim.entityUID env.request.action)) (CedarType.entity Γ.reqty.action.ty)
+  := by
+    constructor
+    simp only [InstanceOfEntityType, hinst_action, true_and]
+    apply Or.inr
+    exact hcontains_action
+  simp only [Env.symbolize?, Request.symbolize?]
+  constructor
+  · constructor
+    · split
+      · repeat
+          rename_i heq
+          split at heq
+          · apply value_symbolize?_wf hinst _ _ _ heq
+            repeat first
+            | exact hwf_princ_ty
+            | exact hwf_action_ty
+            | exact hwf_resource_ty
+            | exact hwf_context_ty
+            | constructor; exact hwf_princ
+            | constructor; exact hwf_action
+            | constructor; exact hwf_resource
+            | exact hwf_context
+            | exact hinst_princ
+            | exact hinst_action
+            | exact hinst_resource
+            | exact hinst_context
+        contradiction
+      · exact defaultLitWithDefaultEid_wf hwf_Γ hwf_var
+    · split
+      · repeat
+          rename_i heq
+          split at heq
+          apply value_symbolize?_is_lit heq
+        contradiction
+      · exact default_lit_is_lit
+  · split
+    · rename_i heq
+      repeat
+        split at heq
+        rename_i heq heq_var
+        simp only [beq_iff_eq] at heq_var
+        simp only [heq_var]
+        apply value_symbolize?_well_typed (Γ := Γ) _ _ heq
+        repeat first
+        | exact hwf_princ_ty
+        | exact hwf_action_ty
+        | exact hwf_resource_ty
+        | exact hwf_context_ty
+        | exact hinst_princ
+        | exact hinst_action
+        | exact hinst_resource
+        | exact hinst_context
+      contradiction
+    · exact default_lit_well_typed
+
+private theorem default_udf_wf
+  {Γ : TypeEnv} {uuf : UUF}
+  (hwf_Γ : Γ.WellFormed)
+  (hwf_uuf : UUF.WellFormed (SymEnv.ofEnv Γ).entities uuf) :
+  Interpretation.WellFormed.WellFormedUUFInterpretation (SymEnv.ofEnv Γ).entities uuf
+    (Decoder.defaultUDF (defaultEidOf Γ) uuf)
+:= by
+  simp only [Decoder.defaultUDF]
+  and_intros
+  · simp only
+    exact defaultLitWithDefaultEid_wf hwf_Γ hwf_uuf.2
+  · simp only
+    exact default_lit_is_lit
+  · simp only
+    exact default_lit_well_typed
+  · simp [Map.empty, Map.WellFormed, Map.toList, Map.kvs, Map.make, List.canonicalize]
+  · simp only
+    intros _ _ h
+    simp [Map.empty, Map.toList, Map.kvs] at h
+  · simp only
+  · simp only
+
+private theorem env_symbolize?_attrs_wf
+  {Γ : TypeEnv} {env : Env}
+  {ety : EntityType} {entry : EntitySchemaEntry}
+  {uuf : UUF} {udf : UDF}
+  (hwf_env : env.StronglyWellFormed)
+  (hinst : InstanceOfWellFormedEnvironment env.request env.entities Γ)
+  (hfind_entry : Map.find? Γ.ets ety = some entry)
+  (hudf : env.entities.symbolizeAttrs? Γ ety entry uuf = some udf) :
+  Interpretation.WellFormed.WellFormedUUFInterpretation
+    (SymEnv.ofEnv Γ).entities uuf udf
+:= by
+  have ⟨_, ⟨hwf_entities, _⟩⟩:= hwf_env
+  have ⟨hwf_Γ, _, hwf_sch⟩ := hinst
+  simp only [
+    Entities.symbolizeAttrs?, beq_iff_eq,
+    Option.ite_none_right_eq_some,
+    Option.some.injEq,
+  ] at hudf
+  simp only [←hudf.2]
+  simp only [Entities.symbolizeAttrs?.udf]
+  have hfind_attrs : Γ.ets.attrs? ety = .some entry.attrs := by
+    simp [EntitySchema.attrs?, hfind_entry]
+  and_intros
+  · simp only
+    apply defaultLitWithDefaultEid_wf hwf_Γ
+    apply ofType_wf hwf_Γ
+    exact wf_env_implies_wf_attrs hwf_Γ hfind_attrs
+  · simp only
+    exact default_lit_is_lit
+  · simp only
+    exact default_lit_well_typed
+  · simp only
+    exact Map.make_wf _
+  -- Well-formed `UDF.table`
+  · simp only
+    intros tᵢ tₒ hmem
+    have hmem := Map.make_mem_list_mem hmem
+    have ⟨⟨uid, data⟩, hmem_uid_data, hio⟩ := List.mem_filterMap.mp hmem
+    have hfind_uid_data := (Map.in_list_iff_find?_some hwf_entities.1).mp hmem_uid_data
+    have ⟨hwf_attrs, _⟩ := hwf_entities.2 uid data hfind_uid_data
+    simp only [bind, Option.bind, Option.ite_none_right_eq_some] at hio
+    have ⟨heq_ety, hio⟩ := hio
+    split at hio
+    contradiction
+    rename_i sym_attrs hsym_attrs
+    simp at hio
+    simp only [←hio]
+    have hwt_attrs : InstanceOfType Γ (Value.record data.attrs) (CedarType.record entry.attrs) := by
+      have := hwf_sch.1 uid data hfind_uid_data
+      simp only [←heq_ety] at hfind_entry
+      cases this with
+      | inl this =>
+        have ⟨_, hfind, _, h, _⟩ := this
+        simp only [hfind_entry, Option.some.injEq] at hfind
+        simp only [←hfind] at h
+        exact h
+      | inr this =>
+        have ⟨_, _, ⟨_, h, _⟩⟩ := this
+        have := wf_env_disjoint_ets_acts hwf_Γ hfind_entry h
+        contradiction
+    have hwf_attrs_ty : CedarType.WellFormed Γ (CedarType.record entry.attrs)
+    := wf_env_implies_wf_attrs hwf_Γ hfind_attrs
+    and_intros
+    · constructor
+      constructor
+      apply env_valid_uid_implies_sym_env_valid_uid hinst
+      exact Map.in_list_implies_contains hmem_uid_data
+    · simp only [←hio.1, Term.isLiteral]
+    · simp only [Term.typeOf, TermPrim.typeOf, TermType.ofType, heq_ety]
+    · apply value_symbolize?_wf hinst hwf_attrs_ty hwf_attrs hwt_attrs hsym_attrs
+    · apply value_symbolize?_is_lit hsym_attrs
+    · apply value_symbolize?_well_typed hwf_attrs_ty hwt_attrs hsym_attrs
+  · simp only [hudf.1]
+  · simp only [hudf.1]
+
+private theorem env_symbolize?_tags_wf
+  {Γ : TypeEnv} {env : Env}
+  {ety : EntityType} {entry : EntitySchemaEntry}
+  {uuf : UUF} {udf : UDF}
+  (hwf_env : env.StronglyWellFormed)
+  (hinst : InstanceOfWellFormedEnvironment env.request env.entities Γ)
+  (hfind_entry : Map.find? Γ.ets ety = some entry)
+  (hudf : env.entities.symbolizeTags? Γ ety entry uuf = some udf) :
+  Interpretation.WellFormed.WellFormedUUFInterpretation
+    (SymEnv.ofEnv Γ).entities uuf udf
+:= by
+  have ⟨_, ⟨hwf_entities, _⟩⟩:= hwf_env
+  have ⟨hwf_Γ, _, hwf_sch⟩ := hinst
+  simp only [Entities.symbolizeTags?, beq_iff_eq, Option.bind_eq_bind] at hudf
+  cases htagTy : entry.tags? with
+  | none => simp [htagTy] at hudf
+  | some tagTy =>
+    have htagTy' : Γ.ets.tags? ety = .some (.some tagTy) := by
+      simp only [EntitySchema.tags?, Option.map_eq_some_iff]
+      exists entry
+    simp only [htagTy, Option.bind_some] at hudf
+    split at hudf
+    -- Tag keys
+    · rename_i hudf_tag_keys
+      simp only [Option.some.injEq] at hudf
+      simp only [
+        ←hudf,
+        Entities.symbolizeTags?.keysUDF,
+      ]
+      and_intros
+      · simp only
+        apply defaultLitWithDefaultEid_wf hwf_Γ
+        apply ofType_wf hwf_Γ
+        repeat constructor
+      · simp only
+        exact default_lit_is_lit
+      · simp only
+        exact default_lit_well_typed
+      · simp only
+        exact Map.make_wf _
+      -- Well-formed `UDF.table`
+      · simp only
+        intros tᵢ tₒ hmem
+        have hmem := Map.make_mem_list_mem hmem
+        have ⟨⟨uid, data⟩, hmem_uid_data, hio⟩ := List.mem_filterMap.mp hmem
+        have hfind_uid_data := (Map.in_list_iff_find?_some hwf_entities.1).mp hmem_uid_data
+        have ⟨hwf_attrs, _⟩ := hwf_entities.2 uid data hfind_uid_data
+        simp only [Option.ite_none_right_eq_some, Option.some.injEq, Prod.mk.injEq] at hio
+        have ⟨heq_ety, hio⟩ := hio
+        simp only [← hio]
+        and_intros
+        · constructor
+          constructor
+          apply env_valid_uid_implies_sym_env_valid_uid hinst
+          exact Map.in_list_implies_contains hmem_uid_data
+        · simp only [Term.isLiteral]
+        · simp only [Term.typeOf, TermPrim.typeOf, TermType.ofType, heq_ety]
+        · constructor
+          · intros t hmem_t
+            replace hmem_t := (Set.make_mem _ _).mpr hmem_t
+            have ⟨_, _, h⟩ := List.mem_map.mp hmem_t
+            simp only [←h]
+            constructor
+            constructor
+          · intros t hmem_t
+            replace hmem_t := (Set.make_mem _ _).mpr hmem_t
+            have ⟨_, _, h⟩ := List.mem_map.mp hmem_t
+            simp only [←h]
+            simp only [Term.typeOf, TermPrim.typeOf]
+          · constructor
+          · exact Set.make_wf _
+        · unfold Term.isLiteral
+          apply List.all_eq_true.mpr
+          intros x hmem_x
+          simp only
+          replace hmem_x := x.property
+          have hmem_x := (Set.make_mem _ _).mpr hmem_x
+          have ⟨_, _, h⟩ := List.mem_map.mp hmem_x
+          simp only [←h, Term.isLiteral]
+        · simp only [Term.typeOf, TermType.ofType]
+      · simp only [hudf_tag_keys]
+      · simp only [hudf_tag_keys]
+    -- Tag values
+    · simp only [Option.ite_none_right_eq_some, Option.some.injEq] at hudf
+      have hudf_tag_vals := hudf.1
+      replace hudf := hudf.2
+      simp only [
+        ←hudf,
+        Entities.symbolizeTags?.valsUDF,
+      ]
+      and_intros
+      · simp only
+        apply defaultLitWithDefaultEid_wf hwf_Γ
+        apply ofType_wf hwf_Γ
+        apply wf_env_implies_wf_tag_type hwf_Γ htagTy'
+      · simp only
+        exact default_lit_is_lit
+      · simp only
+        exact default_lit_well_typed
+      · simp only
+        exact Map.make_wf _
+      · simp only
+        intros tᵢ tₒ hmem
+        have hmem := Map.make_mem_list_mem hmem
+        have ⟨l, hmem_l, hmem⟩ := List.mem_flatten.mp hmem
+        have ⟨⟨uid, data⟩, hmem_uid_data, hl⟩ := List.mem_filterMap.mp hmem_l
+        simp only [Option.bind_eq_bind, Option.ite_none_right_eq_some] at hl
+        have ⟨heq_ety, hl⟩ := hl
+        have ⟨⟨tag, val⟩, hmem_tag_val, htag_val⟩ :=
+          List.mapM_some_implies_all_from_some hl (tᵢ, tₒ) hmem
+        simp only [bind, Option.bind] at htag_val
+        split at htag_val
+        contradiction
+        rename_i sym_val hsym_val
+        simp only [Option.some.injEq, Prod.mk.injEq] at htag_val
+        simp only [←htag_val]
+        have hwf_tagTy : tagTy.WellFormed Γ
+        := wf_env_implies_wf_tag_type hwf_Γ htagTy'
+        have hfind_uid_data := (Map.in_list_iff_find?_some hwf_entities.1).mp hmem_uid_data
+        have ⟨_, _, _, hwf_tags_map, hwf_tags⟩ := hwf_entities.2 uid data hfind_uid_data
+        have hwf_val : val.WellFormed env.entities := by
+          have := (Map.in_list_iff_find?_some hwf_tags_map).mp hmem_tag_val
+          exact hwf_tags tag val this
+        have hwt_val : InstanceOfType Γ val tagTy := by
+          have := hwf_sch.1 uid data hfind_uid_data
+          cases this with
+          | inl this =>
+            have ⟨entry', hfind_entry', _, _, _, h⟩ := this
+            simp only [←heq_ety] at hfind_entry
+            simp only [hfind_entry, Option.some.injEq] at hfind_entry'
+            simp only [InstanceOfEntityTags, ←hfind_entry', htagTy] at h
+            exact h val (Map.in_list_in_values hmem_tag_val)
+          | inr this =>
+            have ⟨_, htag_emp, _⟩ := this
+            simp [htag_emp, Map.empty, Map.toList, Map.kvs] at hmem_tag_val
+        and_intros
+        · constructor
+          · intros a t hmem_a_t
+            simp only [
+              Map.toList, Map.kvs,
+              List.mem_cons, Prod.mk.injEq,
+              List.not_mem_nil, or_false,
+            ] at hmem_a_t
+            cases hmem_a_t with
+            | inl hmem_a_t =>
+              simp only [hmem_a_t]
+              constructor
+              constructor
+              apply env_valid_uid_implies_sym_env_valid_uid hinst
+              exact Map.in_list_implies_contains hmem_uid_data
+            | inr hmem_a_t =>
+              simp only [hmem_a_t]
+              constructor
+              constructor
+          · simp [
+              Map.WellFormed, Map.make,
+              List.canonicalize, Map.toList,
+              Map.kvs, List.insertCanonical,
+            ]
+        · simp [Term.isLiteral, List.all, List.attach₃, List.pmap]
+        · simp only [
+            Term.typeOf, TermPrim.typeOf,
+            TermType.ofType, heq_ety,
+            TermType.tagFor, EntityTag.mk,
+            List.attach₃, List.map, List.pmap,
+          ]
+        · apply value_symbolize?_wf hinst hwf_tagTy hwf_val hwt_val hsym_val
+        · apply value_symbolize?_is_lit hsym_val
+        · apply value_symbolize?_well_typed hwf_tagTy hwt_val hsym_val
+      · simp only [hudf_tag_vals]
+      · simp only [hudf_tag_vals]
+
+private theorem env_symbolize?_ancs_wf
+  {Γ : TypeEnv} {env : Env}
+  {ety : EntityType} {entry : EntitySchemaEntry}
+  {uuf : UUF} {udf : UDF}
+  (hwf_env : env.StronglyWellFormed)
+  (hinst : InstanceOfWellFormedEnvironment env.request env.entities Γ)
+  (hfind_entry : Map.find? Γ.ets ety = some entry)
+  (hudf : env.entities.symbolizeAncs? Γ ety entry uuf = some udf) :
+  Interpretation.WellFormed.WellFormedUUFInterpretation
+    (SymEnv.ofEnv Γ).entities uuf udf
+:= by
+  have ⟨_, ⟨hwf_entities, _⟩⟩:= hwf_env
+  have ⟨hwf_Γ, _, hwf_sch⟩ := hinst
+  simp only [Entities.symbolizeAncs?, beq_iff_eq, Option.bind_eq_bind] at hudf
+  have ⟨_, anc, _, heq, hudf, _⟩ := List.findSome?_eq_some_iff.mp hudf
+  have hmem_ancs : anc ∈ entry.ancestors := by
+    apply (Set.in_list_iff_in_set _ _).mp
+    simp only [Set.toList] at heq
+    simp [heq]
+  simp only [Option.ite_none_right_eq_some, Option.some.injEq] at hudf
+  simp only [←hudf, Entities.symbolizeAncs?.udf]
+  and_intros
+  · simp only
+    apply defaultLitWithDefaultEid_wf hwf_Γ
+    apply ofType_wf hwf_Γ
+    constructor
+    constructor
+    exact wf_env_implies_wf_ancestor hwf_Γ hfind_entry hmem_ancs
+  · simp only
+    exact default_lit_is_lit
+  · simp only
+    exact default_lit_well_typed
+  · simp only
+    exact Map.make_wf _
+  · simp only
+    intros tᵢ tₒ hmem
+    have hmem := Map.make_mem_list_mem hmem
+    have ⟨⟨uid, data⟩, hmem_uid_data, hio⟩ := List.mem_filterMap.mp hmem
+    have hfind_uid_data := (Map.in_list_iff_find?_some hwf_entities.1).mp hmem_uid_data
+    have ⟨_, _, hwf_ancs, _⟩ := hwf_entities.2 uid data hfind_uid_data
+    simp only [Option.ite_none_right_eq_some, Option.some.injEq, Prod.mk.injEq] at hio
+    have ⟨heq_ety, hio⟩ := hio
+    simp only [← hio]
+    and_intros
+    · constructor
+      constructor
+      apply env_valid_uid_implies_sym_env_valid_uid hinst
+      exact Map.in_list_implies_contains hmem_uid_data
+    · simp only [Term.isLiteral]
+    · simp only [Term.typeOf, TermPrim.typeOf, TermType.ofType, heq_ety]
+    · constructor
+      · intros t hmem_t
+        replace hmem_t := (Set.make_mem _ _).mpr hmem_t
+        have ⟨anc, hmem_anc, h⟩ := List.mem_filterMap.mp hmem_t
+        simp only [Option.ite_none_right_eq_some, Option.some.injEq] at h
+        simp only [←h]
+        constructor
+        constructor
+        apply env_valid_uid_implies_sym_env_valid_uid hinst
+        exact hwf_ancs anc hmem_anc
+      · intros t hmem_t
+        replace hmem_t := (Set.make_mem _ _).mpr hmem_t
+        have ⟨anc, hmem_anc, h⟩ := List.mem_filterMap.mp hmem_t
+        simp only [Option.ite_none_right_eq_some, Option.some.injEq] at h
+        simp only [←h, Term.typeOf, TermPrim.typeOf]
+      · constructor
+        apply ofEnv_wf_entity hwf_Γ
+        apply wf_env_implies_wf_ancestor hwf_Γ hfind_entry hmem_ancs
+      · exact Set.make_wf _
+    · unfold Term.isLiteral
+      apply List.all_eq_true.mpr
+      intros x hmem_x
+      simp only
+      replace hmem_x := x.property
+      have hmem_x := (Set.make_mem _ _).mpr hmem_x
+      have ⟨anc, hmem_anc, h⟩ := List.mem_filterMap.mp hmem_x
+      simp only [Option.ite_none_right_eq_some, Option.some.injEq] at h
+      simp only [←h, Term.isLiteral]
+    · simp only [Term.typeOf, TermType.ofType]
+  · simp only [hudf]
+  · simp only [hudf]
+
+private theorem env_symbolize?_wf_funs
+  {Γ : TypeEnv} {env : Env} {uuf : UUF}
+  (hwf_env : env.StronglyWellFormed)
+  (hinst : InstanceOfWellFormedEnvironment env.request env.entities Γ)
+  (hwf_uuf : UUF.WellFormed (SymEnv.ofEnv Γ).entities uuf) :
+  Interpretation.WellFormed.WellFormedUUFInterpretation
+    (SymEnv.ofEnv Γ).entities
+    uuf
+    ((env.symbolize? Γ).funs uuf)
+:= by
+  have ⟨hwf_Γ, _, _⟩ := hinst
+  simp only [Env.symbolize?, Entities.symbolize?]
+  split
+  · rename_i udf hfind_udf
+    have ⟨_, ⟨ety, entry⟩, _, heq, hudf, _⟩ := List.findSome?_eq_some_iff.mp hfind_udf
+    have hmem_entry : (ety, entry) ∈ Γ.ets.toList := by simp [heq]
+    have hfind_entry := (Map.in_list_iff_find?_some (wf_env_implies_wf_ets_map hwf_Γ)).mp hmem_entry
+    simp only [Option.orElse_eq_orElse, Option.orElse_eq_or, Option.or_eq_some_iff] at hudf
+    cases hudf with
+    | inl hudf_attrs => exact env_symbolize?_attrs_wf hwf_env hinst hfind_entry hudf_attrs
+    | inr hudf =>
+      cases hudf.2 with
+      | inl hudf_tags => exact env_symbolize?_tags_wf hwf_env hinst hfind_entry hudf_tags
+      | inr hudf_ancs =>
+        replace hudf_ancs := hudf_ancs.2
+        exact env_symbolize?_ancs_wf hwf_env hinst hfind_entry hudf_ancs
+  · exact default_udf_wf hwf_Γ hwf_uuf
+
+theorem env_symbolize?_wf
+  {Γ : TypeEnv} {env : Env}
+  (hwf_env : env.StronglyWellFormed)
+  (hinst : InstanceOfWellFormedEnvironment env.request env.entities Γ) :
+  (env.symbolize? Γ).WellFormed (SymEnv.ofEnv Γ).entities
+:= by
+  have ⟨hwf_Γ, _, _⟩ := hinst
+  and_intros
+  · intros var hwf_var
+    exact env_symbolize?_wf_vars hwf_env hinst hwf_var
+  · intros uuf hwf_uuf
+    exact env_symbolize?_wf_funs hwf_env hinst hwf_uuf
+  · intros t ht
+    simp only [Env.symbolize?, defaultLitWithDefaultEid]
+    constructor
+    · constructor
+      · exact defaultLitWithDefaultEid_wf hwf_Γ (wfp_term_implies_wf_ty ht)
+      · exact default_lit_is_lit
+    · exact default_lit_well_typed
+
+theorem env_symbolize?_same
+  {Γ : TypeEnv} {env : Env}
+  (hwf_env : env.StronglyWellFormed)
+  (hinst : InstanceOfWellFormedEnvironment env.request env.entities Γ) :
+  env ∼ (SymEnv.ofEnv Γ).interpret (env.symbolize? Γ)
+:= by
+  constructor
+  · exact env_symbolize?_same_request hwf_env hinst
+  · exact env_symbolize?_same_entities hwf_env hinst
+
+theorem ofEnv_soundness
+  {Γ : TypeEnv} {env : Env}
+  (hwf_env : env.StronglyWellFormed)
+  (hinst : InstanceOfWellFormedEnvironment env.request env.entities Γ) :
+  env ∈ᵢ SymEnv.ofEnv Γ
+:= by
+  have ⟨hwf, hinst_req, hinst_sch⟩ := hinst
+  exists env.symbolize? Γ
+  constructor
+  · exact env_symbolize?_wf hwf_env hinst
+  . exact env_symbolize?_same hwf_env hinst
+
+end Cedar.Thm
